\documentclass{report}
\usepackage{amsmath, amssymb, amsthm}
\usepackage{physics}
\usepackage{slashed}
\usepackage{tikz}
\usepackage{tikz-feynman}

\include{shortcut}

\title{Fun with $\gamma$ Matrix}
\author{Weibin Zhang}
\date{2019-04-16}

\begin{document}

%%%%%%%%%%%%%%%%%%%%%%%%%%%%%%%%%%%%%%%%%%%%%%%%%%%%%%%%%%%%%%%%%%%%%%%%
\section{Dirac Equation}

%%%%%%%%%%%%%%%%%%%%%%%%%%%%%%%%%%%%%%%%%%%%%%%%
\subsection{Conplex Conjugate}

%%%%%%%%%%%%%%%%%%%%%%%%%%%%%%%%%%%%%%%%%%%%%%%%
\subsection{$\gamma^5$}
$$ \{\gammaMu, \gammaNu \} = \gammaMu\gammaNu + \gammaNu\gammaMu = 2\eta^{\mn} $$

%%%%%%%%%%%%%%%%%%%%%%%%%%%%%%%%%%%%%%%%%%%%%%%%%%%%%%%%%%%%%%%%%%%%%%%%
\section{Slashed}
\begin{itemize}
    \item $$ \slashed{p}\gammaNu = p_\mu\gammaMu\gammaNu = p_\mu(2\eta^{\mn} - \gammaNu\gammaMu) = 2p^\nu - \gammaNu\slashed{p} $$
	    $$ \Godown $$
	  $$ \slashed{p}\gammaNu + \gammaNu\slashed{p} = 2p^\nu \cdot \CI$$

    \item $$ \slashed{p}\slashed{q} = p_\mu q_\nu \gammaMu\gammaNu = 2pq - \slashed{q}\slashed{p} $$
	    $$ \Godown $$
	  $$ \slashed{p}\slashed{q} + \slashed{q}\slashed{p} = 2pq\cdot \CI $$

    \item $$ \gammaMu\slashed{p}\gammamu = \gammaMu\gammaNu p_\nu\gammamu = (2\eta^{\mn} - \gammaNu\gammaMu)p_\nu \gammamu = 2\slashed{p} - \slashed{p}\gammaMu\gammamu = -2\slashed{p} $$

    \item $$ \gammaMu\slashed{p}\gammaNu\gammamu = (2p^\mu - \slashed{p}\gammaMu)\gammaNu\gammamu = 2\gammaNu\slashed{p} + 2\slashed{p}\gammaNu = 2p^\nu \cdot \CI $$

    \item $$ \gammaMu\slashed{p}\slashed{q}\gammamu = (2p^\mu - \slashed{p}\gammaMu)(2q_\mu - \gammamu\slashed{q}) = 4pq - 2\slashed{p}\slashed{q} - 2\slashed{p}\slashed{q} + 4\slashed{p}\slashed{q} = 4pq\cdot \CI $$

    \item 
	\begin{equation*}
	    \begin{aligned}
		\gammaMu\slashed{p}\gammanu\slashed{q}\gammamu &= (2p^\mu - \slashed{p}\gammaMu)\gammanu(2q_\mu - \gammamu\slashed{q}) = 4pq\gammanu - 2\gammanu\slashed{p}\slashed{q} - 2\slashed{p}\slashed{q}\gammanu + \slashed{p}\gammaMu\gammanu\gammamu\slashed{q}   \\%1
		&= 4pq\gammanu - 2\gammanu\slashed{p}\slashed{q} - 2\slashed{p}\slashed{q}\gammanu - 2\slashed{p}\gammanu\slashed{q}	\\%2
		&= 2\gammanu(2pq - \slashed{p}\slashed{q}) - 2\slashed{p}(\slashed{q}\gammanu + \gammanu\slashed{q})	\\%3
		&= \gammanu 2\slashed{q}\slashed{p} - 4\slashed{p} q_\nu	\\%4
		&= 2(\gammanu\slashed{q} - 2q_\nu)\slashed{p}	\\%5
		&= -2\slashed{q}\gammanu\slashed{p}    \\%6
	    \end{aligned}
	\end{equation*}
\end{itemize}


%%%%%%%%%%%%%%%%%%%%%%%%%%%%%%%%%%%%%%%%%%%%%%%%%%%%%%%%%%%%%%%%%%%%%%%%
\section{Trace}



\end{document}

